theories/lang/cpp/logic/destroy.v
@@ -32,7 +32,7 @@ Section destroy.
       destruct_obj dtor cls this Q
     | Tarray t sz =>
       let destruct_at i :=
-          Exists p, _offsetL (_sub t (Z.of_nat i)) (_eq this) &~ p ** destruct t (Vptr p) dtor empSP
+          Exists p, _offsetL (_sub t (Z.of_nat i)) (_eqv this) &~ p ** destruct t (Vptr p) dtor empSP
       in
       sepSPs (List.map destruct_at (List.seq 0 (N.to_nat sz - 1)))
     | _ => empSP
@@ -44,6 +44,6 @@ Section destroy.
     match dtor with
     | None => fun x => x
     | Some dtor => destruct ty this dtor
-    end (_at (_eq this) (tany (erase_qualifiers ty) 1) ** Q).
+    end (_at (_eqv this) (tany (erase_qualifiers ty) 1) ** Q).
 
 End destroy.
