theories/lang/cpp/logic/initializers.v
@@ -56,8 +56,8 @@ Module Type Init.
       | Tchar _ _
       | Tint _ _ =>
         wp_prval init (fun v free =>
-                         _at (_eq addr) (uninit (erase_qualifiers ty) 1) **
-                         (   _at (_eq addr) (tprim (erase_qualifiers ty) 1 v)
+                         _at (_eqv addr) (uninit (erase_qualifiers ty) 1) **
+                         (   _at (_eqv addr) (tprim (erase_qualifiers ty) 1 v)
                           -* k free))
 
         (* non-primitives are handled via prvalue-initialization semantics *)
@@ -73,7 +73,7 @@ Module Type Init.
 
     Axiom wpi_initialize : forall this_val i cls Q,
         Exists a,
-          _offsetL (offset_for cls i.(init_path)) (_eq this_val) &~ a ** ltrue //\\
+          _offsetL (offset_for cls i.(init_path)) (_eqv this_val) &~ a ** ltrue //\\
         wp_initialize (erase_qualifiers i.(init_type)) (Vptr a) i.(init_init) Q
         |-- wpi cls this_val i Q.
 
@@ -108,9 +108,9 @@ Module Type Init.
       match build_array ls fill (N.to_nat sz) with
       | None => lfalse
       | Some array_list =>
-        _at (_eq addr) (uninit (erase_qualifiers (Tarray ety sz)) 1) **
+        _at (_eqv addr) (uninit (erase_qualifiers (Tarray ety sz)) 1) **
           wps (fun '(i,e) (Q : unit -> mpred -> mpred) f =>
-                 Forall a, _offsetL (_sub ety i) (_eq addr) &~ a -*
+                 Forall a, _offsetL (_sub ety i) (_eqv addr) &~ a -*
                  wp_init ety (Vptr a) e (fun f' => Q tt (f ** f')))
               array_list
               (fun _ free => Q free) empSP
